high2/Zeta.High.Interleave.fst
@@ -1,5 +1,22 @@
 module Zeta.High.Interleave
 
+let blum_evict_elem_props
+  (#app #n:_)
+  (il: verifiable_log app n)
+  (i: seq_index il {is_blum_evict il i})
+  : Lemma (ensures (let e = I.index il i in
+                    let MSD.MHDom (gk,vk) t_e tid_e = blum_evict_elem il i in
+                    let tid = I.src il i in
+                    let st_pre = thread_store_pre tid il i in
+                    let k = V.evict_slot e in
+                    k = to_base_key gk /\
+                    store_contains st_pre k /\
+                    gk = stored_key st_pre k /\
+                    vk = stored_value st_pre k /\
+                    t_e = V.blum_evict_timestamp e /\
+                    tid_e = tid))
+  = admit()
+
 let mk_vlog_entry_ext #app #n (il: verifiable_log app n) (i: seq_index il)
   = let vle = I.index il i in
     let open Zeta.GenericVerifier in
@@ -176,6 +193,13 @@ let ext_evict_val_is_stored_val (#app #n:_) (il: verifiable_log app n) (i: seq_i
                   let bk = V.evict_slot e in
                   store_contains st_pre bk /\
                   HV.stored_value st_pre bk = value_ext ee))
+  = admit()
+
+let ext_blum_timestamp_is_src (#app #n:_) (il: verifiable_log app n) (i: seq_index il)
+  : Lemma (requires (is_blum_evict il i))
+          (ensures (let tid = I.src il i in
+                    let EvictBlum _ _ tid_e = mk_vlog_entry_ext il i in
+                    tid_e = tid))
   = admit()
 
 let ext_app_records_is_stored_val
