high2/Zeta.High.Thread.fsti
@@ -8,16 +8,35 @@ open Zeta.Generic.Thread
 let verifiable_log (app:_)
   = Zeta.Generic.Thread.verifiable_log (high_verifier_spec app)
 
-val lemma_blum_add_elem_key (#app:_) (tl: verifiable_log app) (i: seq_index tl {is_blum_add tl i})
+let store (#app:_) (tl: verifiable_log app)
+  = let vs = state tl in
+    vs.st
+
+let store_pre (#app:_) (tl: verifiable_log app) (i: seq_index tl)
+  = let tl' = prefix tl i in
+    store tl'
+
+let store_post (#app:_) (tl: verifiable_log app) (i: seq_index tl)
+  = let tl' = prefix tl (i+1) in
+    store tl'
+
+val lemma_blum_add_elem_props (#app:_) (tl: verifiable_log app) (i: seq_index tl {is_blum_add tl i})
   : Lemma (ensures (let open Zeta.MultiSetHashDomain in
                     let be = blum_add_elem tl i in
-                    let gk,_ = be.r in
+                    let gk,gv = be.r in
                     add_slot (index tl i) = to_base_key gk))
           [SMTPat (blum_add_elem tl i)]
 
 val lemma_blum_evict_elem_key (#app:_) (tl: verifiable_log app) (i: seq_index tl {is_blum_evict tl i})
   : Lemma (ensures (let open Zeta.MultiSetHashDomain in
+                    let st_pre = store_pre tl i in
                     let be = blum_evict_elem tl i in
-                    let gk,_ = be.r in
-                    evict_slot (index tl i) = to_base_key gk))
+                    let gk,gv = be.r in
+                    let k = evict_slot (index tl i) in
+                    let open Zeta.MultiSetHashDomain in
+                    k = to_base_key gk /\
+                    gk = stored_key st_pre k /\
+                    gv = stored_value st_pre k /\
+                    be.t = blum_evict_timestamp (index tl i) /\
+                    be.tid = fst tl))
           [SMTPat (blum_evict_elem tl i)]
